<?xml version="1.0"?>
<rdf:RDF xmlns="http://data.hulib.helsinki.fi/attx/onto#"
     xml:base="http://data.hulib.helsinki.fi/attx/onto"
     xmlns:cc="https://creativecommons.org/ns#"
     xmlns:rdf="http://www.w3.org/1999/02/22-rdf-syntax-ns#"
     xmlns:owl="http://www.w3.org/2002/07/owl#"
     xmlns:xml="http://www.w3.org/XML/1998/namespace"
     xmlns:xsd="http://www.w3.org/2001/XMLSchema#"
     xmlns:dcterms="http://purl.org/dc/terms/"
     xmlns:pwo="http://purl.org/spar/pwo/"
     xmlns:skos="http://www.w3.org/2004/02/skos/core#"
     xmlns:rdfs="http://www.w3.org/2000/01/rdf-schema#"
     xmlns:prov="http://www.w3.org/ns/prov#"
     xmlns:dc="http://purl.org/dc/elements/1.1/">
    <owl:Ontology rdf:about="http://data.hulib.helsinki.fi/attx/onto#">
        <owl:versionIRI rdf:resource="http://data.hulib.helsinki.fi/attx/onto#"/>
        <rdfs:comment xml:lang="en">This ontology is published by the ATTX project, part of the University of Helsinki Library.</rdfs:comment>
        <owl:versionInfo xml:lang="en">ATTX Workflow ontology 2.0</owl:versionInfo>
        <dc:date>2017-07-04</dc:date>
        <rdfs:seeAlso xml:lang="en">http://helsinki.fi/library</rdfs:seeAlso>
        <dc:creator>ATTX project team</dc:creator>
        <rdfs:label xml:lang="en">ATTX Workflow Ontology</rdfs:label>
        <dc:rights>This work is licensed under a Creative Commons Attribution 4.0 International License.</dc:rights>
        <dc:rights>This work is licensed under a Creative Commons Attribution 4.0 International License http://creativecommons.org/licenses/by/4.0/</dc:rights>
    </owl:Ontology>
    


    <!-- 
    ///////////////////////////////////////////////////////////////////////////////////////
    //
    // Annotation properties
    //
    ///////////////////////////////////////////////////////////////////////////////////////
     -->

    


    <!-- http://purl.org/dc/elements/1.1/creator -->

    <owl:AnnotationProperty rdf:about="http://purl.org/dc/elements/1.1/creator"/>
    


    <!-- http://purl.org/dc/elements/1.1/date -->

    <owl:AnnotationProperty rdf:about="http://purl.org/dc/elements/1.1/date"/>
    


    <!-- http://purl.org/dc/elements/1.1/rights -->

    <owl:AnnotationProperty rdf:about="http://purl.org/dc/elements/1.1/rights"/>
    


    <!-- http://www.w3.org/2000/01/rdf-schema#comment -->

    <owl:AnnotationProperty rdf:about="http://www.w3.org/2000/01/rdf-schema#comment"/>
    


    <!-- http://www.w3.org/2004/02/skos/core#altLabel -->

    <owl:AnnotationProperty rdf:about="http://www.w3.org/2004/02/skos/core#altLabel"/>
    


    <!-- http://www.w3.org/2004/02/skos/core#prefLabel -->

    <owl:AnnotationProperty rdf:about="http://www.w3.org/2004/02/skos/core#prefLabel"/>
    


    <!-- 
    ///////////////////////////////////////////////////////////////////////////////////////
    //
    // Object Properties
    //
    ///////////////////////////////////////////////////////////////////////////////////////
     -->

    


    <!-- http://creativecommons.org/ns#license -->

    <owl:ObjectProperty rdf:about="http://creativecommons.org/ns#license">
        <rdfs:range rdf:resource="http://creativecommons.org/ns#License"/>
        <rdfs:comment xml:lang="en">Associated License for a specific dataset.</rdfs:comment>
    </owl:ObjectProperty>
    


    <!-- http://data.hulib.helsinki.fi/attx/onto#hadRole -->

    <owl:ObjectProperty rdf:about="http://data.hulib.helsinki.fi/attx/onto#hadRole">
        <rdfs:domain rdf:resource="http://www.w3.org/ns/prov#Association"/>
        <rdfs:domain rdf:resource="http://www.w3.org/ns/prov#Influence"/>
        <rdfs:range rdf:resource="http://www.w3.org/ns/prov#Role"/>
    </owl:ObjectProperty>
    


    <!-- http://data.hulib.helsinki.fi/attx/onto#hasAssociatedGraph -->

    <owl:ObjectProperty rdf:about="http://data.hulib.helsinki.fi/attx/onto#hasAssociatedGraph">
        <rdfs:domain rdf:resource="http://data.hulib.helsinki.fi/attx/onto#Step"/>
        <rdfs:range rdf:resource="http://data.hulib.helsinki.fi/attx/onto#Dataset"/>
        <rdfs:comment xml:lang="en">A Step can make use of a certain graph/dataset besides the input graph.</rdfs:comment>
        <rdfs:label xml:lang="en">hasAssociatedGraph</rdfs:label>
    </owl:ObjectProperty>
    


    <!-- http://data.hulib.helsinki.fi/attx/onto#hasStrategyType -->

    <owl:ObjectProperty rdf:about="http://data.hulib.helsinki.fi/attx/onto#hasStrategyType">
        <rdfs:comment xml:lang="en">The current strategy if a derivate of a specific type of Linking Strategy.</rdfs:comment>
    </owl:ObjectProperty>
    


    <!-- http://data.hulib.helsinki.fi/attx/onto#isDependentOn -->

    <owl:ObjectProperty rdf:about="http://data.hulib.helsinki.fi/attx/onto#isDependentOn">
        <rdfs:domain rdf:resource="http://data.hulib.helsinki.fi/attx/onto#Artifact"/>
        <rdfs:range rdf:resource="http://data.hulib.helsinki.fi/attx/onto#Artifact"/>
        <rdfs:comment xml:lang="en">An artifact can be depenednt on other artifacts in order to perform an activity.</rdfs:comment>
        <rdfs:label xml:lang="en">isDependentOn</rdfs:label>
    </owl:ObjectProperty>
    


    <!-- http://data.hulib.helsinki.fi/attx/onto#usesArtifact -->

    <owl:ObjectProperty rdf:about="http://data.hulib.helsinki.fi/attx/onto#usesArtifact">
        <rdfs:subPropertyOf rdf:resource="http://www.w3.org/ns/prov#used"/>
        <rdfs:range rdf:resource="http://data.hulib.helsinki.fi/attx/onto#Artifact"/>
        <rdfs:comment xml:lang="en">An artifact can be used by any type of entity or resource in order to perform certain steps/activities.</rdfs:comment>
        <rdfs:label xml:lang="en">usesArtifact</rdfs:label>
    </owl:ObjectProperty>
    


    <!-- http://data.hulib.helsinki.fi/attx/onto#usesWorkflowExecution -->

    <owl:ObjectProperty rdf:about="http://data.hulib.helsinki.fi/attx/onto#usesWorkflowExecution">
        <rdfs:subPropertyOf rdf:resource="http://www.w3.org/2002/07/owl#topObjectProperty"/>
        <rdfs:domain rdf:resource="http://data.hulib.helsinki.fi/attx/onto#Workflow"/>
        <rdfs:range rdf:resource="http://data.hulib.helsinki.fi/attx/onto#WorkflowExecution"/>
        <rdfs:comment xml:lang="en">Specify the Workflow Execution associated with a current Workflow.</rdfs:comment>
        <rdfs:label xml:lang="en">usesWorkflowExecution</rdfs:label>
    </owl:ObjectProperty>
    


    <!-- http://purl.org/spar/pwo/hasFirstStep -->

    <owl:ObjectProperty rdf:about="http://purl.org/spar/pwo/hasFirstStep">
        <rdfs:domain rdf:resource="http://data.hulib.helsinki.fi/attx/onto#Workflow"/>
        <rdfs:range rdf:resource="http://data.hulib.helsinki.fi/attx/onto#Step"/>
        <rdfs:comment xml:lang="en">A workflow that starts with a particular step.</rdfs:comment>
        <rdfs:label xml:lang="en">has first step</rdfs:label>
    </owl:ObjectProperty>
    


    <!-- http://purl.org/spar/pwo/hasNextStep -->

    <owl:ObjectProperty rdf:about="http://purl.org/spar/pwo/hasNextStep">
        <rdfs:domain rdf:resource="http://data.hulib.helsinki.fi/attx/onto#Step"/>
        <rdfs:range rdf:resource="http://data.hulib.helsinki.fi/attx/onto#Step"/>
        <rdfs:comment xml:lang="en">A property linking a step in a workflow with the step that directly follows it.</rdfs:comment>
        <rdfs:label xml:lang="en">has next step</rdfs:label>
    </owl:ObjectProperty>
    


    <!-- http://purl.org/spar/pwo/hasStep -->

    <owl:ObjectProperty rdf:about="http://purl.org/spar/pwo/hasStep">
        <rdfs:domain rdf:resource="http://data.hulib.helsinki.fi/attx/onto#Workflow"/>
        <rdfs:range rdf:resource="http://data.hulib.helsinki.fi/attx/onto#Step"/>
        <rdfs:comment xml:lang="en">The property linking a workflow to a component step.</rdfs:comment>
        <rdfs:label xml:lang="en">has step</rdfs:label>
    </owl:ObjectProperty>
    


    <!-- http://www.w3.org/ns/prov#agent -->

    <owl:ObjectProperty rdf:about="http://www.w3.org/ns/prov#agent">
        <rdfs:range rdf:resource="http://www.w3.org/ns/prov#Agent"/>
        <rdfs:comment xml:lang="en">The prov:agent property references an prov:Agent which influenced a resource. This property applies to an prov:AgentInfluence, which is given by a subproperty of prov:qualifiedInfluence from the influenced prov:Entity, prov:Activity or prov:Agent.</rdfs:comment>
        <rdfs:label xml:lang="en">agent</rdfs:label>
    </owl:ObjectProperty>
    


    <!-- http://www.w3.org/ns/prov#generated -->

    <owl:ObjectProperty rdf:about="http://www.w3.org/ns/prov#generated">
        <rdfs:domain rdf:resource="http://www.w3.org/ns/prov#Activity"/>
        <rdfs:comment xml:lang="en">Generation is the completion of production of a new entity by an activity. This entity did not exist before generation and becomes available for usage after this generation.</rdfs:comment>
        <rdfs:label xml:lang="en">generated</rdfs:label>
    </owl:ObjectProperty>
    


    <!-- http://www.w3.org/ns/prov#hadDerivation -->

    <owl:ObjectProperty rdf:about="http://www.w3.org/ns/prov#hadDerivation">
        <owl:inverseOf rdf:resource="http://www.w3.org/ns/prov#wasDerivedFrom"/>
        <rdfs:comment xml:lang="en">Inverse of wasDerivedFrom property</rdfs:comment>
        <rdfs:label xml:lang="en">hadDerivation</rdfs:label>
    </owl:ObjectProperty>
    


    <!-- http://www.w3.org/ns/prov#hadPlan -->

    <owl:ObjectProperty rdf:about="http://www.w3.org/ns/prov#hadPlan">
        <rdfs:domain rdf:resource="http://www.w3.org/ns/prov#Association"/>
        <rdfs:range rdf:resource="http://www.w3.org/ns/prov#Plan"/>
        <rdfs:comment xml:lang="en">A plan is an entity that represents a set of actions or steps intended by one or more agents to achieve some goals.</rdfs:comment>
        <rdfs:label xml:lang="en">hadPlan</rdfs:label>
    </owl:ObjectProperty>
    


    <!-- http://www.w3.org/ns/prov#qualifiedAssociation -->

    <owl:ObjectProperty rdf:about="http://www.w3.org/ns/prov#qualifiedAssociation">
        <rdfs:comment xml:lang="en">An activity association is an assignment of responsibility to an agent for an activity, indicating that the agent had a role in the activity. It further allows for a plan to be specified, which is the plan intended by the agent to achieve some goals in the context of this activity.</rdfs:comment>
        <rdfs:label xml:lang="en">qualifiedAssociation</rdfs:label>
    </owl:ObjectProperty>
    


    <!-- http://www.w3.org/ns/prov#used -->

    <owl:ObjectProperty rdf:about="http://www.w3.org/ns/prov#used">
        <rdfs:domain rdf:resource="http://www.w3.org/ns/prov#Activity"/>
        <rdfs:comment xml:lang="en">Usage is the beginning of utilizing an entity by an activity. Before usage, the activity had not begun to utilize this entity and could not have been affected by the entity.</rdfs:comment>
        <rdfs:label xml:lang="en">used</rdfs:label>
    </owl:ObjectProperty>
    


    <!-- http://www.w3.org/ns/prov#wasAssociatedWith -->

    <owl:ObjectProperty rdf:about="http://www.w3.org/ns/prov#wasAssociatedWith">
        <rdfs:domain rdf:resource="http://www.w3.org/ns/prov#Activity"/>
        <rdfs:range rdf:resource="http://www.w3.org/ns/prov#Agent"/>
        <rdfs:comment xml:lang="en">An activity association is an assignment of responsibility to an agent for an activity, indicating that the agent had a role in the activity. It further allows for a plan to be specified, which is the plan intended by the agent to achieve some goals in the context of this activity.</rdfs:comment>
        <rdfs:label xml:lang="en">wasAssociatedWith</rdfs:label>
    </owl:ObjectProperty>
    


    <!-- http://www.w3.org/ns/prov#wasDerivedFrom -->

    <owl:ObjectProperty rdf:about="http://www.w3.org/ns/prov#wasDerivedFrom">
        <rdfs:comment xml:lang="en">A derivation is a transformation of an entity into another, an update of an entity resulting in a new one, or the construction of a new entity based on a pre-existing entity.</rdfs:comment>
        <rdfs:label xml:lang="en">wasDerivedFrom</rdfs:label>
    </owl:ObjectProperty>
    


    <!-- http://www.w3.org/ns/prov#wasGeneratedBy -->

    <owl:ObjectProperty rdf:about="http://www.w3.org/ns/prov#wasGeneratedBy">
        <rdfs:comment xml:lang="en">Generation is the completion of production of a new entity by an activity. This entity did not exist before generation and becomes available for usage after this generation.</rdfs:comment>
        <rdfs:label xml:lang="en">wasGeneratedBy</rdfs:label>
    </owl:ObjectProperty>
    


    <!-- 
    ///////////////////////////////////////////////////////////////////////////////////////
    //
    // Data properties
    //
    ///////////////////////////////////////////////////////////////////////////////////////
     -->

    


    <!-- http://data.hulib.helsinki.fi/attx/onto#hasStepConfig -->

    <owl:DatatypeProperty rdf:about="http://data.hulib.helsinki.fi/attx/onto#hasStepConfig">
        <rdfs:comment xml:lang="en">A Step can have different configurations associated to with which specifies the Workflow how to perform the given step.</rdfs:comment>
        <rdfs:label xml:lang="en">hasStepConfig</rdfs:label>
    </owl:DatatypeProperty>
    


    <!-- http://www.w3.org/ns/prov#endedAtTime -->

    <owl:DatatypeProperty rdf:about="http://www.w3.org/ns/prov#endedAtTime">
        <rdfs:domain rdf:resource="http://www.w3.org/ns/prov#Activity"/>
        <rdfs:range rdf:resource="http://www.w3.org/2001/XMLSchema#dateTime"/>
        <rdfs:comment xml:lang="en">End is when an activity is deemed to have been ended by an entity, known as trigger. The activity no longer exists after its end. Any usage, generation, or invalidation involving an activity precedes the activity&apos;s end. An end may refer to a trigger entity that terminated the activity, or to an activity, known as ender that generated the trigger.</rdfs:comment>
        <rdfs:label xml:lang="en">endedAtTime</rdfs:label>
    </owl:DatatypeProperty>
    


    <!-- http://www.w3.org/ns/prov#startedAtTime -->

    <owl:DatatypeProperty rdf:about="http://www.w3.org/ns/prov#startedAtTime">
        <rdfs:domain rdf:resource="http://www.w3.org/ns/prov#Activity"/>
        <rdfs:range rdf:resource="http://www.w3.org/2001/XMLSchema#dateTime"/>
        <rdfs:comment xml:lang="en">Start is when an activity is deemed to have been started by an entity, known as trigger. The activity did not exist before its start. Any usage, generation, or invalidation involving an activity follows the activity&apos;s start. A start may refer to a trigger entity that set off the activity, or to an activity, known as starter, that generated the trigger.</rdfs:comment>
        <rdfs:label xml:lang="en">startedAtTime</rdfs:label>
    </owl:DatatypeProperty>
    


    <!-- 
    ///////////////////////////////////////////////////////////////////////////////////////
    //
    // Classes
    //
    ///////////////////////////////////////////////////////////////////////////////////////
     -->

    


    <!-- http://creativecommons.org/ns#License -->

    <owl:Class rdf:about="http://creativecommons.org/ns#License">
        <rdfs:comment xml:lang="en">A set of requests/permissions to users of a Work, e.g. a copyright license, the public domain, information for distributors</rdfs:comment>
        <rdfs:label xml:lang="en">License</rdfs:label>
    </owl:Class>
    


    <!-- http://data.hulib.helsinki.fi/attx/onto#AcquisitionWorkflow -->

    <owl:Class rdf:about="http://data.hulib.helsinki.fi/attx/onto#AcquisitionWorkflow">
        <rdfs:subClassOf rdf:resource="http://data.hulib.helsinki.fi/attx/onto#Workflow"/>
        <rdfs:comment xml:lang="en">A sequence of dependent steps, with the main goal of acquiring/importing/accessing information from a specific source.</rdfs:comment>
        <rdfs:label xml:lang="en">Acquisition Workflow</rdfs:label>
    </owl:Class>
    


    <!-- http://data.hulib.helsinki.fi/attx/onto#Artifact -->

    <owl:Class rdf:about="http://data.hulib.helsinki.fi/attx/onto#Artifact">
        <rdfs:subClassOf rdf:resource="http://www.w3.org/ns/prov#SoftwareAgent"/>
        <rdfs:comment xml:lang="en">An artifact is a type of mutable or imutable resource used in a specific workflow. Examples: Web Service, source code or any other type of software component and not only.</rdfs:comment>
        <rdfs:label xml:lang="en">Artifact</rdfs:label>
    </owl:Class>
    


    <!-- http://data.hulib.helsinki.fi/attx/onto#Dataset -->

    <owl:Class rdf:about="http://data.hulib.helsinki.fi/attx/onto#Dataset">
        <rdfs:comment xml:lang="en">A specific resource which represents a Dataset used in an workflow.</rdfs:comment>
        <rdfs:label xml:lang="en">Dataset</rdfs:label>
    </owl:Class>
    


    <!-- http://data.hulib.helsinki.fi/attx/onto#DisseminationWorkflow -->

    <owl:Class rdf:about="http://data.hulib.helsinki.fi/attx/onto#DisseminationWorkflow">
        <rdfs:subClassOf rdf:resource="http://data.hulib.helsinki.fi/attx/onto#Workflow"/>
        <rdfs:comment xml:lang="en">A sequence of dependent steps, representing a series of activities that make it possible to publish and distribute information (e.g. via an API).</rdfs:comment>
        <rdfs:label xml:lang="en">Dissemination Workflow</rdfs:label>
    </owl:Class>
    


    <!-- http://data.hulib.helsinki.fi/attx/onto#DistributionStep -->

    <owl:Class rdf:about="http://data.hulib.helsinki.fi/attx/onto#DistributionStep">
        <rdfs:subClassOf rdf:resource="http://data.hulib.helsinki.fi/attx/onto#Step"/>
        <rdfs:comment xml:lang="en">A specif action/type of activity performed in an Workflow, that has associated an output (always a Working Data Graph) at the end of the Workflow.</rdfs:comment>
        <rdfs:label xml:lang="en">Distribution Step</rdfs:label>
    </owl:Class>
    


    <!-- http://data.hulib.helsinki.fi/attx/onto#EnrichmentWorkflow -->

    <owl:Class rdf:about="http://data.hulib.helsinki.fi/attx/onto#EnrichmentWorkflow">
        <rdfs:subClassOf rdf:resource="http://data.hulib.helsinki.fi/attx/onto#Workflow"/>
        <rdfs:comment xml:lang="en">A sequence steps that have the main purpose of enriching information from a specific Dataset. The act of enriching can be performed by a specific artifact and can vary from simple linkage and/or adding new properties to complex inferecing.</rdfs:comment>
        <rdfs:label xml:lang="en">Enrichment Workflow</rdfs:label>
    </owl:Class>
    


    <!-- http://data.hulib.helsinki.fi/attx/onto#InputStep -->

    <owl:Class rdf:about="http://data.hulib.helsinki.fi/attx/onto#InputStep">
        <rdfs:subClassOf rdf:resource="http://data.hulib.helsinki.fi/attx/onto#Step"/>
        <rdfs:comment xml:lang="en">A specif action/type of activity performed in an Workflow, that has associated an input (always a Data Graph) at the beginning of the Workflow.</rdfs:comment>
        <rdfs:label xml:lang="en">Input Step</rdfs:label>
    </owl:Class>
    


    <!-- http://data.hulib.helsinki.fi/attx/onto#LinkingStrategy -->

    <owl:Class rdf:about="http://data.hulib.helsinki.fi/attx/onto#LinkingStrategy">
        <rdfs:comment xml:lang="en">A Linking Strategy represents an operation or a set of operations with different parameters that has the purpose to connection two or more datasets. There can be multiple types of strategies (e.g. IDs strategy, NER, etc.), each type of strategy having multiple and distinct types of parameters (e.g. for SPARQL we can add parameters for the type of skos predicate to be used; for NER we can add multiple languages or training sets etc.).</rdfs:comment>
        <rdfs:label xml:lang="en">Linking Strategy</rdfs:label>
    </owl:Class>
    


    <!-- http://data.hulib.helsinki.fi/attx/onto#Process -->

    <owl:Class rdf:about="http://data.hulib.helsinki.fi/attx/onto#Process">
        <rdfs:comment xml:lang="en">Process refers to an activity or series of actions (steps) caused by Agents, performed via a Worfklow and resulting in new Datasets.</rdfs:comment>
        <rdfs:label xml:lang="en">Process</rdfs:label>
    </owl:Class>
    


    <!-- http://data.hulib.helsinki.fi/attx/onto#ProcessingStep -->

    <owl:Class rdf:about="http://data.hulib.helsinki.fi/attx/onto#ProcessingStep">
        <rdfs:subClassOf rdf:resource="http://data.hulib.helsinki.fi/attx/onto#Step"/>
        <rdfs:comment xml:lang="en">A specif action/type of activity performed in an Workflow, that registeres Metadata specific information about the current Workflow. This Step can be performed imediately after the InputStep or at any other point in the Workflow but not after the OutputStep.</rdfs:comment>
        <rdfs:label xml:lang="en">Processing Step</rdfs:label>
    </owl:Class>
    


    <!-- http://data.hulib.helsinki.fi/attx/onto#Step -->

    <owl:Class rdf:about="http://data.hulib.helsinki.fi/attx/onto#Step">
        <rdfs:subClassOf rdf:resource="http://www.w3.org/ns/prov#Activity"/>
        <rdfs:comment xml:lang="en">A specif action/type of activity performed in an Workflow, that may have associated a start time and an end time, and may be associated with one or more Artifacts.</rdfs:comment>
        <rdfs:label xml:lang="en">Step</rdfs:label>
    </owl:Class>
    


    <!-- http://data.hulib.helsinki.fi/attx/onto#Workflow -->

    <owl:Class rdf:about="http://data.hulib.helsinki.fi/attx/onto#Workflow">
        <rdfs:subClassOf rdf:resource="http://www.w3.org/ns/prov#Plan"/>
        <rdfs:comment xml:lang="en">A sequence of dependent steps, representing a series of activities that make use of certain Artifacts and Datasets. A workflow is performed as part of a specific Plan and has associated a WorkflowExecution activity.</rdfs:comment>
        <rdfs:label xml:lang="en">Workflow</rdfs:label>
    </owl:Class>
    


    <!-- http://data.hulib.helsinki.fi/attx/onto#WorkflowExecution -->

    <owl:Class rdf:about="http://data.hulib.helsinki.fi/attx/onto#WorkflowExecution">
        <rdfs:subClassOf rdf:resource="http://www.w3.org/ns/prov#Activity"/>
        <rdfs:comment xml:lang="en">A workflow execution represents the execution of a Workflow and is itself an Activity. The execution process can also describe the specific artifacts used to acomplish the Workflow, the Dataset and Agent described in the proces template.</rdfs:comment>
        <rdfs:label xml:lang="en">Workflow Execution</rdfs:label>
    </owl:Class>
    


    <!-- http://www.w3.org/ns/prov#Activity -->

    <owl:Class rdf:about="http://www.w3.org/ns/prov#Activity">
        <rdfs:comment xml:lang="en">An activity is something that occurs over a period of time and acts upon or with entities; it may include consuming, processing, transforming, modifying, relocating, using, or generating entities.</rdfs:comment>
        <rdfs:label xml:lang="en">Activity</rdfs:label>
    </owl:Class>
    


    <!-- http://www.w3.org/ns/prov#Agent -->

    <owl:Class rdf:about="http://www.w3.org/ns/prov#Agent">
        <rdfs:comment xml:lang="en">An agent is something that bears some form of responsibility for an activity taking place, for the existence of an entity, or for another agent&apos;s activity.</rdfs:comment>
        <rdfs:label xml:lang="en">Agent</rdfs:label>
    </owl:Class>
    


    <!-- http://www.w3.org/ns/prov#Association -->

    <owl:Class rdf:about="http://www.w3.org/ns/prov#Association">
        <rdfs:comment xml:lang="en">An activity association is an assignment of responsibility to an agent for an activity, indicating that the agent had a role in the activity. It further allows for a plan to be specified, which is the plan intended by the agent to achieve some goals in the context of this activity.</rdfs:comment>
        <rdfs:label xml:lang="en">Association</rdfs:label>
    </owl:Class>
    


    <!-- http://www.w3.org/ns/prov#Influence -->

    <owl:Class rdf:about="http://www.w3.org/ns/prov#Influence">
        <rdfs:comment xml:lang="en">Influence is the capacity of an entity, activity, or agent to have an effect on the character, development, or behavior of another by means of usage, start, end, generation, invalidation, communication, derivation, attribution, association, or delegation.</rdfs:comment>
        <rdfs:label xml:lang="en">Influence</rdfs:label>
    </owl:Class>
    


    <!-- http://www.w3.org/ns/prov#Plan -->

    <owl:Class rdf:about="http://www.w3.org/ns/prov#Plan">
        <rdfs:comment xml:lang="en">A plan is an entity that represents a set of actions or steps intended by one or more agents to achieve some goals.</rdfs:comment>
        <rdfs:comment xml:lang="en">There exist no prescriptive requirement on the nature of plans, their representation, the actions or steps they consist of, or their intended goals. Since plans may evolve over time, it may become necessary to track their provenance, so plans themselves are entities. Representing the plan explicitly in the provenance can be useful for various tasks: for example, to validate the execution as represented in the provenance record, to manage expectation failures, or to provide explanations.</rdfs:comment>
        <rdfs:label xml:lang="en">Plan</rdfs:label>
    </owl:Class>
    


    <!-- http://www.w3.org/ns/prov#Role -->

    <owl:Class rdf:about="http://www.w3.org/ns/prov#Role">
        <rdfs:comment xml:lang="en">A role is the function of an entity or agent with respect to an activity, in the context of a usage, generation, invalidation, association, start, and end.</rdfs:comment>
        <rdfs:label xml:lang="en">Role</rdfs:label>
    </owl:Class>
    


    <!-- http://www.w3.org/ns/prov#SoftwareAgent -->

    <owl:Class rdf:about="http://www.w3.org/ns/prov#SoftwareAgent">
        <rdfs:subClassOf rdf:resource="http://www.w3.org/ns/prov#Agent"/>
        <rdfs:comment xml:lang="en">A software agent is running software.</rdfs:comment>
        <rdfs:label xml:lang="en">SoftwareAgent</rdfs:label>
    </owl:Class>
    


    <!-- 
    ///////////////////////////////////////////////////////////////////////////////////////
    //
    // Individuals
    //
    ///////////////////////////////////////////////////////////////////////////////////////
     -->

    


    <!-- http://data.hulib.helsinki.fi/attx/onto#CC0 -->

    <owl:NamedIndividual rdf:about="http://data.hulib.helsinki.fi/attx/onto#CC0">
        <rdf:type rdf:resource="http://creativecommons.org/ns#License"/>
        <rdfs:comment>CC0
“No Rights Reserved”</rdfs:comment>
        <rdfs:label>CreativeCommons 0</rdfs:label>
    </owl:NamedIndividual>
    


    <!-- http://data.hulib.helsinki.fi/attx/onto#Unknown -->

    <owl:NamedIndividual rdf:about="http://data.hulib.helsinki.fi/attx/onto#Unknown">
        <rdf:type rdf:resource="http://creativecommons.org/ns#License"/>
        <rdfs:comment xml:lang="en">An Unknown license type, this means the license might contain copyrighted work.</rdfs:comment>
        <rdfs:label xml:lang="en">Unknown</rdfs:label>
    </owl:NamedIndividual>
</rdf:RDF>



<!-- Generated by the OWL API (version 4.2.8.20170104-2310) https://github.com/owlcs/owlapi -->

